<script>
MathJax = {
  tex: {
    inlineMath: [['$', '$'], ['\\(', '\\)']]
  }
};
</script>
<script id="MathJax-script" async
  src="https://cdn.jsdelivr.net/npm/mathjax@3/es5/tex-chtml.js">
</script>

# 10.2.2

If $f:[a,b] \rightarrow \mathbb{R}$ is a constant function, say $f(s) = c$ for every $x \in [a,b]$, show that

---

$Proof$:

Let $f(x) = c$ for all $x \in [a, b]$. Then,

$$
\int_a^b f(x) \, dx = \int_a^b c \, dx
$$

Since $c$ is a constant, it can be factored out of the integral:

$$
\int_a^b c \, dx = c \int_a^b 1 \, dx
$$

Using the fundamental integral formula:

$$
\int_a^b 1 \, dx = b - a
$$

Thus,

$$
c \int_a^b 1 \, dx = c(b - a)
$$

Therefore,

$$
\int_a^b f(x) \, dx = c(b - a)
$$

$\square$

(Iâ€™m not sure whether the explanation above is entirely correct. If you happen to notice any mistakes, I would really appreciate it if you could leave your suggestions in the comments when you have a moment. Thank you very much for your help and corrections.)

<script src="https://giscus.app/client.js"
        data-repo="charlestsaur/charlestsaur.github.io"
        data-repo-id="R_kgDOKvWJJA"
        data-category="Announcements"
        data-category-id="DIC_kwDOKvWJJM4CyE4o"
        data-mapping="pathname"
        data-strict="0"
        data-reactions-enabled="1"
        data-emit-metadata="0"
        data-input-position="bottom"
        data-theme="preferred_color_scheme"
        data-lang="en"
        crossorigin="anonymous"
        async>
</script>
